# 扩展欧几里得

## 思路和推导

!!! info "裴蜀定理"

    $ax + by = c$ 有解 当且仅当 $\gcd(a, b) | c$。

求解 $ax + by = \gcd(a, b)$：

$$
\begin{aligned}
ax + by = \gcd(a, b) = \gcd(b, a \bmod b)\\
bx' + (a \bmod b)y' = \gcd(b, a \bmod b)\\
bx' + (a - \left\lfloor \frac{a}{b} \right\rfloor \times b)y' = \gcd(b, a \bmod b)\\
ay' + b(x' - \left\lfloor \frac{a}{b} \right\rfloor y') = \gcd(b, a\bmod b)
\end{aligned}
$$

因此，我们只需要计算

$$bx' + (a \bmod b)y' = \gcd(b, a \bmod b)$$

的解，就计算出了

$$\left\{\begin{array}{l} x \gets y' \\ y \gets x' - \left\lfloor \frac{a}{b} \right\rfloor y' \end{array}\right.$$

递归的边界为：

当 $b | a$ 时，方程为 $ax + by = b$，解得 $x = 0,\: y = 1$。

## 实现

```cpp
void exgcd(int a, int b, int &x, int &y) {
    if(a % b == 0) x = 0, y = 1;
    else {
        exgcd(b, a % b, y, x);
        y -= a / b * x;
    }
}
```
